v.0902
- use the new compiler to update HSM2FSM case study

UnitTestingDriver/testDriver.py
@@ -18,7 +18,7 @@ Proj2 = "../_ER2REL/"			# task 2
 Proj3 = "../_ResolveTemp/"		# task 3
 
 # PROJ TO VERIFY
-Projs = [Proj3]	
+Projs = [Proj1]	
 
 # WHAT OPTION TO VERIFY EACH PROJ
 Projs_option_map = { Proj1: { _OPT_VALIDATION, _OPT_VERIFICATION}, 
