_HSM2FSM/ATL_Rule_Encoding/IS2IS_matchAll.bpl
@@ -21,15 +21,20 @@ getTarsBySrcs(Seq#Singleton(is1)) !=null
   free ensures $HeapSucc(old($linkHeap), $linkHeap);
   free ensures surj_tar_model($srcHeap, $tarHeap);
 
+function printGuard_IS2IS(hp: HeapType, is1: ref): bool
+{  read(hp, is1, HSM$AbstractState.compositeState)==null  }
 
-implementation IS2IS_matchAllTest () returns ()
+
+
+implementation IS2IS_matchAllTest() returns ()
 {
 
 var stk: Seq BoxType;
-var $i: int;
+var $newCol: ref;
 var is1: ref;	//slot: 1
 var self: ref;	//slot: 0
 var obj#4: Seq ref;
+var $counter#5: int;
 var cond#11: bool;
 var obj#16: ref;
 var obj#28: ref;
@@ -41,36 +46,20 @@ call stk := OpCode#Findme(stk);
 call stk := OpCode#Push(stk, _IN);
 call stk, obj#4 := LIB#AllInstanceFrom(stk, $srcHeap);
 obj#4 := $Unbox(Seq#Index(stk, Seq#Length(stk)-1));
-$i:=0;
+$counter#5:=0;
 call stk := OpCode#Pop(stk);
-while($i<Seq#Length(obj#4))
-	  invariant $i<=Seq#Length(obj#4);
-	  invariant (forall _is1: ref ::
-		_is1!=null && read($srcHeap, _is1, alloc) && dtype(_is1) <: HSM$InitialState ==> Seq#Contains(obj#4,_is1));
-	  invariant (forall i: int:: 0<=i &&i <$i ==>
-			true ==>
-			(
-				Seq#Index(obj#4,i)!=null && read($srcHeap, Seq#Index(obj#4,i), alloc) && dtype(Seq#Index(obj#4,i)) <: HSM$InitialState ==> 
-					read($srcHeap, Seq#Index(obj#4,i), HSM$AbstractState.compositeState)==null  ==>
-					getTarsBySrcs(Seq#Singleton(Seq#Index(obj#4,i)))!=null 
-					&& read($tarHeap, getTarsBySrcs(Seq#Singleton(Seq#Index(obj#4,i))), alloc)
-					&& dtype(getTarsBySrcs(Seq#Singleton(Seq#Index(obj#4,i)))) <: FSM$InitialState
-			)
-		);
-	  invariant (forall<alpha> $o : ref, $f: Field alpha ::
-	($o == null 
-	|| read($tarHeap, $o, $f) == read(old($tarHeap), $o, $f) 
-	|| ((dtype($o) <: FSM$InitialState) && Seq#Length(getTarsBySrcs_inverse($o)) == 1 && dtype(Seq#Index(getTarsBySrcs_inverse($o), 0)) <: HSM$InitialState && $f==alloc )));
-      free invariant $HeapSucc(old($tarHeap), $tarHeap);
-      free invariant $HeapSucc(old($linkHeap), $linkHeap);
-{ 
-stk := Seq#Build(stk, $Box(Seq#Index(obj#4, $i)));
+while($counter#5<Seq#Length(obj#4)) 
+invariant $counter#5 <= Seq#Length(obj#4);
+invariant (forall _is1: ref :: _is1 != null && read($srcHeap, _is1, alloc) && dtype(_is1) <: HSM$InitialState ==> Seq#Contains(obj#4,_is1));
+invariant (forall _$counter#5: int :: 0<= _$counter#5 && _$counter#5< $counter#5 ==> true ==> (Seq#Index(obj#4,_$counter#5)!=null && read($srcHeap, Seq#Index(obj#4,_$counter#5), alloc) && dtype(Seq#Index(obj#4,_$counter#5)) <: HSM$InitialState ==>printGuard_IS2IS($srcHeap,Seq#Index(obj#4,_$counter#5)) ==> getTarsBySrcs(Seq#Singleton(Seq#Index(obj#4,_$counter#5))) != null &&read($tarHeap, getTarsBySrcs(Seq#Singleton(Seq#Index(obj#4,_$counter#5))), alloc) && dtype(getTarsBySrcs(Seq#Singleton(Seq#Index(obj#4,_$counter#5)))) <: FSM$InitialState));
+invariant (forall<alpha> $o : ref, $f: Field alpha :: ($o == null || read($tarHeap, $o, $f) == read(old($tarHeap), $o, $f) || ((dtype($o) <: FSM$InitialState) && Seq#Length(getTarsBySrcs_inverse($o)) == 1 && dtype(Seq#Index(getTarsBySrcs_inverse($o), 0)) <: HSM$InitialState && $f==alloc )));
+{ stk := Seq#Build(stk, $Box(Seq#Index(obj#4, $counter#5)));
 call stk, is1 := OpCode#Store(stk);
 call stk := OpCode#Load(stk, is1);
 assert Seq#Length(stk) >= 1;
 assert $Unbox(Seq#Index(stk, Seq#Length(stk)-1)) != null;
 assert read($srcHeap, $Unbox(Seq#Index(stk, Seq#Length(stk)-1)),alloc);
-stk := Seq#Build(Seq#Take(stk, Seq#Length(stk)-1), $Box(read($srcHeap,$Unbox(Seq#Index(stk, Seq#Length(stk)-1)),FieldOfDecl(dtype($Unbox(Seq#Index(stk, Seq#Length(stk)-1))), _Field$compositeState): Field (ref))));
+stk := Seq#Build(Seq#Take(stk, Seq#Length(stk)-1), $Box(read($srcHeap,$Unbox(Seq#Index(stk, Seq#Length(stk)-1)),HSM$AbstractState.compositeState)));
 call stk := OCLAny#IsUndefined(stk);
 call stk := OCL#Boolean#Not(stk);
 cond#11 := $Unbox(Seq#Index(stk, Seq#Length(stk)-1));
@@ -80,8 +69,7 @@ label_12:
 call stk := OpCode#GetASM(stk);
 assert Seq#Length(stk) >= 1;
 assert $Unbox(Seq#Index(stk, Seq#Length(stk)-1)) != null;
-assert read($linkHeap, $Unbox(Seq#Index(stk, Seq#Length(stk)-1)),alloc);
-stk := Seq#Build(Seq#Take(stk, Seq#Length(stk)-1), $Box(read($linkHeap,$Unbox(Seq#Index(stk, Seq#Length(stk)-1)),FieldOfDecl(dtype($Unbox(Seq#Index(stk, Seq#Length(stk)-1))), _Field$links): Field (Set ref))));
+stk := Seq#Build(Seq#Take(stk, Seq#Length(stk)-1), $Box(read($linkHeap,$Unbox(Seq#Index(stk, Seq#Length(stk)-1)),ASM.links)));
 call stk := OpCode#Push(stk, _TransientLink);
 call stk := OpCode#Push(stk, _#native);
 assert Seq#Length(stk) >= 2;
@@ -116,7 +104,7 @@ call stk := NTransientLink#addTargetElement(stk,$Unbox(Seq#Index(stk, Seq#Length
 call stk := OpCode#Pusht(stk);
 stk := Seq#Take(stk, Seq#Length(stk)-3);
 label_32:
-$i := $i+1;
+$counter#5 := $counter#5+1;
 }
 
 }
