_HSM2FSM/ATL_Rule_Encoding/RS2RS_matchAll.bpl
@@ -21,15 +21,20 @@ getTarsBySrcs(Seq#Singleton(rs1)) !=null
   free ensures $HeapSucc(old($linkHeap), $linkHeap);
   free ensures surj_tar_model($srcHeap, $tarHeap);
 
+function printGuard_RS2RS(hp: HeapType, rs1: ref): bool
+{  true  }
+
   
-implementation RS2RS_matchAllTest () returns ()
+
+implementation RS2RS_matchAllTest() returns ()
 {
 
 var stk: Seq BoxType;
-var $i: int;
+var $newCol: ref;
 var rs1: ref;	//slot: 1
 var self: ref;	//slot: 0
 var obj#4: Seq ref;
+var $counter#5: int;
 var obj#11: ref;
 var obj#23: ref;
 stk := OpCode#Aux#InitStk();
@@ -40,68 +45,54 @@ call stk := OpCode#Findme(stk);
 call stk := OpCode#Push(stk, _IN);
 call stk, obj#4 := LIB#AllInstanceFrom(stk, $srcHeap);
 obj#4 := $Unbox(Seq#Index(stk, Seq#Length(stk)-1));
-$i:=0;
+$counter#5:=0;
 call stk := OpCode#Pop(stk);
-while($i<Seq#Length(obj#4))
-	  invariant $i<=Seq#Length(obj#4);
-	  invariant (forall _rs1: ref ::
-		_rs1!=null && read($srcHeap, _rs1, alloc) && dtype(_rs1) <: HSM$RegularState ==> Seq#Contains(obj#4,_rs1));
-	  invariant (forall i: int:: 0<=i &&i <$i ==>
-			true ==>
-			(
-				Seq#Index(obj#4,i)!=null && read($srcHeap, Seq#Index(obj#4,i), alloc) && dtype(Seq#Index(obj#4,i)) <: HSM$RegularState ==> 
-					getTarsBySrcs(Seq#Singleton(Seq#Index(obj#4,i)))!=null 
-					&& read($tarHeap, getTarsBySrcs(Seq#Singleton(Seq#Index(obj#4,i))), alloc)
-					&& dtype(getTarsBySrcs(Seq#Singleton(Seq#Index(obj#4,i)))) <: FSM$RegularState
-			)
-		);
-	  invariant (forall<alpha> $o : ref, $f: Field alpha ::
-	($o == null || read($tarHeap, $o, $f) == read(old($tarHeap), $o, $f) || (dtype($o) <: FSM$RegularState && Seq#Length(getTarsBySrcs_inverse($o)) == 1 && dtype(Seq#Index(getTarsBySrcs_inverse($o), 0)) <: HSM$RegularState && $f==alloc)));
-      free invariant $HeapSucc(old($tarHeap), $tarHeap);
-      free invariant $HeapSucc(old($linkHeap), $linkHeap);
-{ 
-	stk := Seq#Build(stk, $Box(Seq#Index(obj#4, $i)));
-	call stk, rs1 := OpCode#Store(stk);
-	call stk := OpCode#GetASM(stk);
-	assert Seq#Length(stk) >= 1;
-	assert $Unbox(Seq#Index(stk, Seq#Length(stk)-1)) != null;
-	assert read($linkHeap, $Unbox(Seq#Index(stk, Seq#Length(stk)-1)),alloc);
-	assert dtype($Unbox(Seq#Index(stk, Seq#Length(stk)-1))) <: System.reserved;
-	stk := Seq#Build(Seq#Take(stk, Seq#Length(stk)-1), $Box(read($linkHeap,$Unbox(Seq#Index(stk, Seq#Length(stk)-1)),FieldOfDecl(dtype($Unbox(Seq#Index(stk, Seq#Length(stk)-1))), _Field$links): Field (Set ref))));
-	call stk := OpCode#Push(stk, _TransientLink);
-	call stk := OpCode#Push(stk, _#native);
-	assert Seq#Length(stk) >= 2;
-	havoc obj#11;
-	assume obj#11!= null && !read($linkHeap, obj#11, alloc) && dtype(obj#11) == classifierTable[($Unbox(Seq#Index(stk, Seq#Length(stk)-1)): String),($Unbox(Seq#Index(stk, Seq#Length(stk)-2)): String)];
-	$linkHeap := update($linkHeap, obj#11, alloc, true);
-	assume $IsGoodHeap($linkHeap);
-	assume $HeapSucc(old($linkHeap), $linkHeap);
-	stk := Seq#Build(Seq#Take(stk, Seq#Length(stk)-2), $Box(obj#11));
+while($counter#5<Seq#Length(obj#4)) 
+invariant $counter#5 <= Seq#Length(obj#4);
+invariant (forall _rs1: ref :: _rs1 != null && read($srcHeap, _rs1, alloc) && dtype(_rs1) <: HSM$RegularState ==> Seq#Contains(obj#4,_rs1));
+invariant (forall _$counter#5: int :: 0<= _$counter#5 && _$counter#5< $counter#5 ==> true ==> (Seq#Index(obj#4,_$counter#5)!=null && read($srcHeap, Seq#Index(obj#4,_$counter#5), alloc) && dtype(Seq#Index(obj#4,_$counter#5)) <: HSM$RegularState ==>printGuard_RS2RS($srcHeap,Seq#Index(obj#4,_$counter#5)) ==> getTarsBySrcs(Seq#Singleton(Seq#Index(obj#4,_$counter#5))) != null &&read($tarHeap, getTarsBySrcs(Seq#Singleton(Seq#Index(obj#4,_$counter#5))), alloc) && dtype(getTarsBySrcs(Seq#Singleton(Seq#Index(obj#4,_$counter#5)))) <: FSM$RegularState));
+invariant (forall<alpha> $o : ref, $f: Field alpha :: ($o == null || read($tarHeap, $o, $f) == read(old($tarHeap), $o, $f) || ((dtype($o) <: FSM$RegularState) && Seq#Length(getTarsBySrcs_inverse($o)) == 1 && dtype(Seq#Index(getTarsBySrcs_inverse($o), 0)) <: HSM$RegularState && $f==alloc )));
+{ stk := Seq#Build(stk, $Box(Seq#Index(obj#4, $counter#5)));
+call stk, rs1 := OpCode#Store(stk);
+call stk := OpCode#GetASM(stk);
+assert Seq#Length(stk) >= 1;
+assert $Unbox(Seq#Index(stk, Seq#Length(stk)-1)) != null;
+stk := Seq#Build(Seq#Take(stk, Seq#Length(stk)-1), $Box(read($linkHeap,$Unbox(Seq#Index(stk, Seq#Length(stk)-1)),ASM.links)));
+call stk := OpCode#Push(stk, _TransientLink);
+call stk := OpCode#Push(stk, _#native);
+assert Seq#Length(stk) >= 2;
+havoc obj#11;
+assume obj#11!= null && !read($linkHeap, obj#11, alloc) && dtype(obj#11) == classifierTable[($Unbox(Seq#Index(stk, Seq#Length(stk)-1)): String),($Unbox(Seq#Index(stk, Seq#Length(stk)-2)): String)];
+$linkHeap := update($linkHeap, obj#11, alloc, true);
+assume $IsGoodHeap($linkHeap);
+assume $HeapSucc(old($linkHeap), $linkHeap);
+stk := Seq#Build(Seq#Take(stk, Seq#Length(stk)-2), $Box(obj#11));
 
-	call stk := OpCode#Dup(stk);
-	call stk := OpCode#Push(stk, _RS2RS);
-	call stk := NTransientLink#setRule(stk,$Unbox(Seq#Index(stk, Seq#Length(stk)-2)),$Unbox(Seq#Index(stk, Seq#Length(stk)-1)));
-	call stk := OpCode#Dup(stk);
-	call stk := OpCode#Push(stk, _rs1);
-	call stk := OpCode#Load(stk, rs1);
-	call stk := NTransientLink#addSourceElement(stk,$Unbox(Seq#Index(stk, Seq#Length(stk)-3)),$Unbox(Seq#Index(stk, Seq#Length(stk)-2)),$Unbox(Seq#Index(stk, Seq#Length(stk)-1)));
-	call stk := OpCode#Dup(stk);
-	call stk := OpCode#Push(stk, _rs2);
-	call stk := OpCode#Push(stk, _RegularState);
-	call stk := OpCode#Push(stk, _FSM);
-	assert Seq#Length(stk) >= 2;
-	havoc obj#23;
-	assume obj#23!= null && !read($tarHeap, obj#23, alloc) && dtype(obj#23) == classifierTable[($Unbox(Seq#Index(stk, Seq#Length(stk)-1)): String),($Unbox(Seq#Index(stk, Seq#Length(stk)-2)): String)];
-	$tarHeap := update($tarHeap, obj#23, alloc, true);
-	assume $IsGoodHeap($tarHeap);
-	assume $HeapSucc(old($tarHeap), $tarHeap);
-	assume getTarsBySrcs(Seq#Singleton(rs1)) == obj#23;
-	stk := Seq#Build(Seq#Take(stk, Seq#Length(stk)-2), $Box(obj#23));
+call stk := OpCode#Dup(stk);
+call stk := OpCode#Push(stk, _RS2RS);
+call stk := NTransientLink#setRule(stk,$Unbox(Seq#Index(stk, Seq#Length(stk)-2)),$Unbox(Seq#Index(stk, Seq#Length(stk)-1)));
+call stk := OpCode#Dup(stk);
+call stk := OpCode#Push(stk, _rs1);
+call stk := OpCode#Load(stk, rs1);
+call stk := NTransientLink#addSourceElement(stk,$Unbox(Seq#Index(stk, Seq#Length(stk)-3)),$Unbox(Seq#Index(stk, Seq#Length(stk)-2)),$Unbox(Seq#Index(stk, Seq#Length(stk)-1)));
+call stk := OpCode#Dup(stk);
+call stk := OpCode#Push(stk, _rs2);
+call stk := OpCode#Push(stk, _RegularState);
+call stk := OpCode#Push(stk, _FSM);
+assert Seq#Length(stk) >= 2;
+havoc obj#23;
+assume obj#23!= null && !read($tarHeap, obj#23, alloc) && dtype(obj#23) == classifierTable[($Unbox(Seq#Index(stk, Seq#Length(stk)-1)): String),($Unbox(Seq#Index(stk, Seq#Length(stk)-2)): String)];
+$tarHeap := update($tarHeap, obj#23, alloc, true);
+assume $IsGoodHeap($tarHeap);
+assume $HeapSucc(old($tarHeap), $tarHeap);
+assume getTarsBySrcs(Seq#Singleton(rs1)) == obj#23;
+stk := Seq#Build(Seq#Take(stk, Seq#Length(stk)-2), $Box(obj#23));
 
-	call stk := NTransientLink#addTargetElement(stk,$Unbox(Seq#Index(stk, Seq#Length(stk)-3)),$Unbox(Seq#Index(stk, Seq#Length(stk)-2)),$Unbox(Seq#Index(stk, Seq#Length(stk)-1)));
-	call stk := OpCode#Pusht(stk);
-	stk := Seq#Take(stk, Seq#Length(stk)-3);
-	$i := $i+1;
+call stk := NTransientLink#addTargetElement(stk,$Unbox(Seq#Index(stk, Seq#Length(stk)-3)),$Unbox(Seq#Index(stk, Seq#Length(stk)-2)),$Unbox(Seq#Index(stk, Seq#Length(stk)-1)));
+call stk := OpCode#Pusht(stk);
+stk := Seq#Take(stk, Seq#Length(stk)-3);
+$counter#5 := $counter#5+1;
 }
 
 }
+
