_HSM2FSM/ATL_Rule_Encoding/SM2SM_applyAll.bpl
@@ -1,6 +1,6 @@
 procedure SM2SM_applyAllTest() returns();
-requires surj_tar_model($srcHeap, $tarHeap);
-requires (forall sm1: ref :: sm1!=null && read($srcHeap, sm1, alloc) && dtype(sm1) <: HSM$StateMachine 
+  requires surj_tar_model($srcHeap, $tarHeap);
+  requires (forall sm1: ref :: sm1!=null && read($srcHeap, sm1, alloc) && dtype(sm1) <: HSM$StateMachine 
  ==>
  true  ==>
 getTarsBySrcs(Seq#Singleton(sm1)) !=null 
@@ -8,14 +8,19 @@ getTarsBySrcs(Seq#Singleton(sm1)) !=null
 && dtype(getTarsBySrcs(Seq#Singleton(sm1))) <: FSM$StateMachine);
   modifies $tarHeap;
 // Rule outcome
+
+
   ensures (forall sm1: ref :: sm1!=null && read($srcHeap, sm1, alloc) && dtype(sm1) <: HSM$StateMachine 
  ==>
  true  ==>
 read($tarHeap, getTarsBySrcs(Seq#Singleton(sm1)), FSM$StateMachine.name) == read($srcHeap, sm1, HSM$StateMachine.name));
+
+
 // Frame property
   ensures (forall<alpha> $o: ref, $f: Field alpha :: 
 	!read(old($tarHeap), $o, alloc) ==>
-		 ( read($tarHeap, $o, $f) == read(old($tarHeap), $o, $f)));
+		 ( read($tarHeap, $o, $f) == read(old($tarHeap), $o, $f))
+	  || (dtype($o) == class._System.array));
   ensures (forall<alpha> $o: ref, $f: Field alpha :: 
 	$o != null && read(old($tarHeap), $o, alloc) ==>
 		(Seq#Length(getTarsBySrcs_inverse($o)) == 1 && dtype(Seq#Index(getTarsBySrcs_inverse($o), 0)) <: HSM$StateMachine && ( dtype($o) <: FSM$StateMachine && ($f == FSM$StateMachine.name))) 
@@ -46,7 +51,8 @@ implementation SM2SM_applyAllTest () returns ()
 		);
 		invariant (forall<alpha> $o: ref, $f: Field alpha :: 
 	!read(old($tarHeap), $o, alloc) ==>
-		 ( read($tarHeap, $o, $f) == read(old($tarHeap), $o, $f)));
+		 ( read($tarHeap, $o, $f) == read(old($tarHeap), $o, $f))
+	  || (dtype($o) == class._System.array));
 	{
 		link := Seq#Index(links, $i);		
 		call SM2SM_apply(link);
@@ -57,40 +63,59 @@ implementation SM2SM_applyAllTest () returns ()
 }
 
 
-procedure SM2SM_apply (in: ref) returns ();
-  free requires surj_tar_model($srcHeap, $tarHeap);
-  free requires $linkHeap[in, TransientLink#rule]==_SM2SM;  
-  free requires $linkHeap[in, alloc] == true;
-  free requires dtype(in) <: Native$TransientLink;
-  free requires Map#Domain($linkHeap[in, TransientLink#source])[_sm1];
-  free requires Map#Domain($linkHeap[in, TransientLink#target])[_sm2];
-  free requires dtype(Map#Elements($linkHeap[in, TransientLink#source])[_sm1]) <:HSM$StateMachine;
-  free requires Map#Elements($linkHeap[in, TransientLink#source])[_sm1] != null;
-  free requires read($srcHeap,Map#Elements($linkHeap[in, TransientLink#source])[_sm1],alloc);
-  free requires dtype(Map#Elements($linkHeap[in, TransientLink#target])[_sm2]) <: FSM$StateMachine;
-  free requires Map#Elements($linkHeap[in, TransientLink#target])[_sm2] != null;
-  free requires read($tarHeap,Map#Elements($linkHeap[in, TransientLink#target])[_sm2],alloc);
-  free requires getTarsBySrcs(Seq#Singleton(Map#Elements($linkHeap[in, TransientLink#source])[_sm1])) == Map#Elements($linkHeap[in, TransientLink#target])[_sm2];
-  modifies $tarHeap;
-  ensures read($tarHeap, getTarsBySrcs(Seq#Singleton(Map#Elements($linkHeap[in, TransientLink#source])[_sm1])), FSM$StateMachine.name) == read($srcHeap,Map#Elements($linkHeap[in, TransientLink#source])[_sm1],HSM$StateMachine.name);
-  ensures (forall<alpha> $o: ref, $f: Field alpha :: 
+procedure SM2SM_apply(in: ref) returns();
+free requires surj_tar_model($srcHeap, $tarHeap);
+//free requires isValidSrc($srcHeap);
+//free requires isInstTar($tarHeap);
+// link info
+free requires $linkHeap[in, alloc] == true;
+free requires dtype(in) == Native$TransientLink;
+// rule info
+free requires $linkHeap[in, TransientLink#rule]==_SM2SM;  
+free requires Map#Domain($linkHeap[in, TransientLink#source])[_sm1];
+free requires dtype(Map#Elements($linkHeap[in, TransientLink#source])[_sm1]) <: HSM$StateMachine;
+free requires Map#Elements($linkHeap[in, TransientLink#source])[_sm1] != null;
+free requires read($srcHeap, Map#Elements($linkHeap[in, TransientLink#source])[_sm1], alloc);
+
+free requires Map#Domain($linkHeap[in, TransientLink#target])[_sm2];
+free requires dtype(Map#Elements($linkHeap[in, TransientLink#target])[_sm2]) <: FSM$StateMachine;
+free requires Map#Elements($linkHeap[in, TransientLink#target])[_sm2] != null;
+free requires read($tarHeap, Map#Elements($linkHeap[in, TransientLink#target])[_sm2], alloc);
+
+// Correspondence I/O
+free requires getTarsBySrcs(Seq#Singleton(Map#Elements($linkHeap[in, TransientLink#source])[_sm1])) == Map#Elements($linkHeap[in, TransientLink#target])[_sm2];
+// Guard
+free requires true ;
+// modifies
+modifies $tarHeap;
+// Rule outcome
+
+ensures read($tarHeap, getTarsBySrcs(Seq#Singleton(Map#Elements($linkHeap[in, TransientLink#source])[_sm1])), FSM$StateMachine.name) == read($srcHeap, Map#Elements($linkHeap[in, TransientLink#source])[_sm1], HSM$StateMachine.name);
+
+
+// Frame 
+ensures (forall<alpha> $o: ref, $f: Field alpha :: 
+	!read(old($tarHeap), $o, alloc) ==>
+		 ( read($tarHeap, $o, $f) == read(old($tarHeap), $o, $f))
+	  || (dtype($o) == class._System.array));
+ensures (forall<alpha> $o: ref, $f: Field alpha :: 
 	$o != null && read(old($tarHeap), $o, alloc) ==>
-		((dtype($o) <: FSM$StateMachine && dtype(Seq#Index(getTarsBySrcs_inverse($o), 0)) <: HSM$StateMachine && $f == FSM$StateMachine.name) || (read($tarHeap, $o, $f) == read(old($tarHeap), $o, $f))));
-  ensures (forall<alpha> $o: ref, $f: Field alpha :: 
+		(Seq#Length(getTarsBySrcs_inverse($o)) == 1 && dtype(Seq#Index(getTarsBySrcs_inverse($o), 0)) <: HSM$StateMachine && ( dtype($o) <: FSM$StateMachine && ($f == FSM$StateMachine.name))) 
+		|| (read($tarHeap, $o, $f) == read(old($tarHeap), $o, $f)));
+ensures (forall<alpha> $o: ref, $f: Field alpha :: 
 	$o != null && read(old($tarHeap), $o, alloc) && $o != getTarsBySrcs(Seq#Singleton(Map#Elements($linkHeap[in, TransientLink#source])[_sm1])) ==> 
 	(read($tarHeap, $o, $f) == read(old($tarHeap), $o, $f))
-  );	
-  ensures $HeapSucc(old($tarHeap), $tarHeap);
-  ensures surj_tar_model($srcHeap, $tarHeap);
-  ensures (forall<alpha> $o: ref, $f: Field alpha :: 
-	!read(old($tarHeap), $o, alloc) ==>
-		 ( read($tarHeap, $o, $f) == read(old($tarHeap), $o, $f)));
+  );
+// Preserving
+ensures $HeapSucc(old($tarHeap), $tarHeap);
+ensures surj_tar_model($srcHeap, $tarHeap);
   
+
 implementation SM2SM_apply (in: ref) returns ()
 {
 
 var stk: Seq BoxType;
-var $i: int;
+var $newCol: ref;
 var sm2: ref;	//slot: 3
 var sm1: ref;	//slot: 2
 var self: ref;	//slot: 0
@@ -100,44 +125,32 @@ link := in;
 
 call stk := OpCode#Load(stk, link);
 call stk := OpCode#Push(stk, _sm1);
-call stk := NTransientLink#getSourceElement(
-				stk,
-				$Unbox(Seq#Index(stk, Seq#Length(stk)-2)),
-				$Unbox(Seq#Index(stk, Seq#Length(stk)-1)));
+call stk := NTransientLink#getSourceElement(stk,$Unbox(Seq#Index(stk, Seq#Length(stk)-2)),$Unbox(Seq#Index(stk, Seq#Length(stk)-1)));
 call stk, sm1 := OpCode#Store(stk);
 call stk := OpCode#Load(stk, link);
 call stk := OpCode#Push(stk, _sm2);
-call stk := NTransientLink#getTargetElement(
-				stk,
-				$Unbox(Seq#Index(stk, Seq#Length(stk)-2)),
-				$Unbox(Seq#Index(stk, Seq#Length(stk)-1)));
+call stk := NTransientLink#getTargetElement(stk,$Unbox(Seq#Index(stk, Seq#Length(stk)-2)),$Unbox(Seq#Index(stk, Seq#Length(stk)-1)));
 call stk, sm2 := OpCode#Store(stk);
 call stk := OpCode#Load(stk, sm2);
 call stk := OpCode#Dup(stk);
 call stk := OpCode#GetASM(stk);
 call stk := OpCode#Load(stk, sm1);
-
 assert Seq#Length(stk) >= 1;
 assert $Unbox(Seq#Index(stk, Seq#Length(stk)-1)) != null;
 assert read($srcHeap, $Unbox(Seq#Index(stk, Seq#Length(stk)-1)),alloc);
-assert dtype($Unbox(Seq#Index(stk, Seq#Length(stk)-1))) <: HSM$StateMachine;
-stk := Seq#Build(Seq#Take(stk, Seq#Length(stk)-1), $Box(read($srcHeap,$Unbox(Seq#Index(stk, Seq#Length(stk)-1)),FieldOfDecl(dtype($Unbox(Seq#Index(stk, Seq#Length(stk)-1))), _Field$name): Field (String))));
-
+stk := Seq#Build(Seq#Take(stk, Seq#Length(stk)-1), $Box(read($srcHeap,$Unbox(Seq#Index(stk, Seq#Length(stk)-1)),HSM$StateMachine.name)));
 call stk := ASM#Resolve(stk, $srcHeap, $Unbox(Seq#Index(stk, Seq#Length(stk)-1)): String);
-
 assert Seq#Length(stk) >= 2;
 assert $Unbox(Seq#Index(stk, Seq#Length(stk)-2)) != null;
 assert read($tarHeap, $Unbox(Seq#Index(stk, Seq#Length(stk)-2)), alloc);
-assert dtype($Unbox(Seq#Index(stk, Seq#Length(stk)-2))) <: FSM$StateMachine;
-$tarHeap := update($tarHeap, $Unbox(Seq#Index(stk, Seq#Length(stk)-2)), 
-				FieldOfDecl(dtype($Unbox(Seq#Index(stk, Seq#Length(stk)-2))), _Field$name): Field (String), 
-				$Unbox(Seq#Index(stk, Seq#Length(stk)-1)));
+$tarHeap := update($tarHeap, $Unbox(Seq#Index(stk, Seq#Length(stk)-2)),FSM$StateMachine.name,$Unbox(Seq#Index(stk, Seq#Length(stk)-1)));
 assume $IsGoodHeap($tarHeap);
 stk := Seq#Take(stk, Seq#Length(stk)-2);
 
 call stk := OpCode#Pop(stk);
 
 }
+
 
 
 // properties of each link of e2r rule
