_HSM2FSM/ATL_Rule_Encoding/T2TA_matchAll.bpl
@@ -20,56 +20,45 @@ getTarsBySrcs(Seq#Singleton(t1)) !=null
   free ensures $HeapSucc(old($tarHeap), $tarHeap);
   free ensures $HeapSucc(old($linkHeap), $linkHeap);
   free ensures surj_tar_model($srcHeap, $tarHeap);
+
+function printGuard_T2TA(hp: HeapType, t1: ref): bool
+{  !(dtype(read(hp, t1, HSM$Transition.source)) == HSM$CompositeState) && !(dtype(read(hp, t1, HSM$Transition.target)) == HSM$CompositeState)  }
   
-implementation T2TA_matchAllTest () returns ()
+
+implementation T2TA_matchAllTest() returns ()
 {
 
-	var stk: Seq BoxType;
-	var $i: int;
-	var t1: ref;	//slot: 1
-	var self: ref;	//slot: 0
-	var obj#4: Seq ref;
-	var cond#23: bool;
-	var obj#28: ref;
-	var obj#40: ref;
-	stk := OpCode#Aux#InitStk();
+var stk: Seq BoxType;
+var $newCol: ref;
+var t1: ref;	//slot: 1
+var self: ref;	//slot: 0
+var obj#4: Seq ref;
+var $counter#5: int;
+var cond#23: bool;
+var obj#28: ref;
+var obj#40: ref;
+stk := OpCode#Aux#InitStk();
 
-	call stk := OpCode#Push(stk, _Transition);
-	call stk := OpCode#Push(stk, _HSM);
-	call stk := OpCode#Findme(stk);
-	call stk := OpCode#Push(stk, _IN);
-	call stk, obj#4 := LIB#AllInstanceFrom(stk, $srcHeap);
-	obj#4 := $Unbox(Seq#Index(stk, Seq#Length(stk)-1));
-	$i:=0;
-	call stk := OpCode#Pop(stk);
-	while($i<Seq#Length(obj#4))
-	  invariant $i<=Seq#Length(obj#4);
-	  invariant (forall _t1: ref ::
-		_t1!=null && read($srcHeap, _t1, alloc) && dtype(_t1) <: HSM$Transition ==> Seq#Contains(obj#4,_t1));
-	  invariant (forall i: int:: 0<=i &&i <$i ==>
-			true ==>
-			(
-				Seq#Index(obj#4,i)!=null && read($srcHeap, Seq#Index(obj#4,i), alloc) && dtype(Seq#Index(obj#4,i)) <: HSM$Transition ==> 
-				 !(dtype(read($srcHeap, Seq#Index(obj#4,i), HSM$Transition.source)) == HSM$CompositeState) && !(dtype(read($srcHeap, Seq#Index(obj#4,i), HSM$Transition.target)) == HSM$CompositeState)  ==>
-					getTarsBySrcs(Seq#Singleton(Seq#Index(obj#4,i)))!=null 
-					&& read($tarHeap, getTarsBySrcs(Seq#Singleton(Seq#Index(obj#4,i))), alloc)
-					&& dtype(getTarsBySrcs(Seq#Singleton(Seq#Index(obj#4,i)))) <: FSM$Transition
-			)
-		);
-	  invariant (forall<alpha> $o : ref, $f: Field alpha ::
-	($o == null 
-	|| read($tarHeap, $o, $f) == read(old($tarHeap), $o, $f) 
-	|| ((dtype($o) <: FSM$Transition) && Seq#Length(getTarsBySrcs_inverse($o)) == 1 && dtype(Seq#Index(getTarsBySrcs_inverse($o), 0)) <: HSM$Transition && $f==alloc )));
-      free invariant $HeapSucc(old($tarHeap), $tarHeap);
-      free invariant $HeapSucc(old($linkHeap), $linkHeap);
-	{ 
-stk := Seq#Build(stk, $Box(Seq#Index(obj#4, $i)));
+call stk := OpCode#Push(stk, _Transition);
+call stk := OpCode#Push(stk, _HSM);
+call stk := OpCode#Findme(stk);
+call stk := OpCode#Push(stk, _IN);
+call stk, obj#4 := LIB#AllInstanceFrom(stk, $srcHeap);
+obj#4 := $Unbox(Seq#Index(stk, Seq#Length(stk)-1));
+$counter#5:=0;
+call stk := OpCode#Pop(stk);
+while($counter#5<Seq#Length(obj#4)) 
+invariant $counter#5 <= Seq#Length(obj#4);
+invariant (forall _t1: ref :: _t1 != null && read($srcHeap, _t1, alloc) && dtype(_t1) <: HSM$Transition ==> Seq#Contains(obj#4,_t1));
+invariant (forall _$counter#5: int :: 0<= _$counter#5 && _$counter#5< $counter#5 ==> true ==> (Seq#Index(obj#4,_$counter#5)!=null && read($srcHeap, Seq#Index(obj#4,_$counter#5), alloc) && dtype(Seq#Index(obj#4,_$counter#5)) <: HSM$Transition ==>printGuard_T2TA($srcHeap,Seq#Index(obj#4,_$counter#5)) ==> getTarsBySrcs(Seq#Singleton(Seq#Index(obj#4,_$counter#5))) != null &&read($tarHeap, getTarsBySrcs(Seq#Singleton(Seq#Index(obj#4,_$counter#5))), alloc) && dtype(getTarsBySrcs(Seq#Singleton(Seq#Index(obj#4,_$counter#5)))) <: FSM$Transition));
+invariant (forall<alpha> $o : ref, $f: Field alpha :: ($o == null || read($tarHeap, $o, $f) == read(old($tarHeap), $o, $f) || ((dtype($o) <: FSM$Transition) && Seq#Length(getTarsBySrcs_inverse($o)) == 1 && dtype(Seq#Index(getTarsBySrcs_inverse($o), 0)) <: HSM$Transition && $f==alloc )));
+{ stk := Seq#Build(stk, $Box(Seq#Index(obj#4, $counter#5)));
 call stk, t1 := OpCode#Store(stk);
 call stk := OpCode#Load(stk, t1);
 assert Seq#Length(stk) >= 1;
 assert $Unbox(Seq#Index(stk, Seq#Length(stk)-1)) != null;
 assert read($srcHeap, $Unbox(Seq#Index(stk, Seq#Length(stk)-1)),alloc);
-stk := Seq#Build(Seq#Take(stk, Seq#Length(stk)-1), $Box(read($srcHeap,$Unbox(Seq#Index(stk, Seq#Length(stk)-1)),FieldOfDecl(dtype($Unbox(Seq#Index(stk, Seq#Length(stk)-1))), _Field$source): Field (ref))));
+stk := Seq#Build(Seq#Take(stk, Seq#Length(stk)-1), $Box(read($srcHeap,$Unbox(Seq#Index(stk, Seq#Length(stk)-1)),HSM$Transition.source)));
 call stk := OpCode#Push(stk, _CompositeState);
 call stk := OpCode#Push(stk, _HSM);
 call stk := OpCode#Findme(stk);
@@ -79,10 +68,9 @@ call stk := OpCode#Load(stk, t1);
 assert Seq#Length(stk) >= 1;
 assert $Unbox(Seq#Index(stk, Seq#Length(stk)-1)) != null;
 assert read($srcHeap, $Unbox(Seq#Index(stk, Seq#Length(stk)-1)),alloc);
-stk := Seq#Build(Seq#Take(stk, Seq#Length(stk)-1), $Box(read($srcHeap,$Unbox(Seq#Index(stk, Seq#Length(stk)-1)),FieldOfDecl(dtype($Unbox(Seq#Index(stk, Seq#Length(stk)-1))), _Field$target): Field (ref))));
+stk := Seq#Build(Seq#Take(stk, Seq#Length(stk)-1), $Box(read($srcHeap,$Unbox(Seq#Index(stk, Seq#Length(stk)-1)),HSM$Transition.target)));
 call stk := OpCode#Push(stk, _CompositeState);
 call stk := OpCode#Push(stk, _HSM);
-assert ($Unbox(Seq#Index(stk, Seq#Length(stk)-2))) == _CompositeState;
 call stk := OpCode#Findme(stk);
 call stk := OCLAny#IsTypeof(stk);
 call stk := OCLAny#Not(stk);
@@ -95,8 +83,7 @@ label_24:
 call stk := OpCode#GetASM(stk);
 assert Seq#Length(stk) >= 1;
 assert $Unbox(Seq#Index(stk, Seq#Length(stk)-1)) != null;
-assert read($linkHeap, $Unbox(Seq#Index(stk, Seq#Length(stk)-1)),alloc);
-stk := Seq#Build(Seq#Take(stk, Seq#Length(stk)-1), $Box(read($linkHeap,$Unbox(Seq#Index(stk, Seq#Length(stk)-1)),FieldOfDecl(dtype($Unbox(Seq#Index(stk, Seq#Length(stk)-1))), _Field$links): Field (Set ref))));
+stk := Seq#Build(Seq#Take(stk, Seq#Length(stk)-1), $Box(read($linkHeap,$Unbox(Seq#Index(stk, Seq#Length(stk)-1)),ASM.links)));
 call stk := OpCode#Push(stk, _TransientLink);
 call stk := OpCode#Push(stk, _#native);
 assert Seq#Length(stk) >= 2;
@@ -131,7 +118,7 @@ call stk := NTransientLink#addTargetElement(stk,$Unbox(Seq#Index(stk, Seq#Length
 call stk := OpCode#Pusht(stk);
 stk := Seq#Take(stk, Seq#Length(stk)-3);
 label_44:
-$i := $i+1;
-	}
+$counter#5 := $counter#5+1;
+}
 
 }
