_HSM2FSM/ExecutionSemantics/ATLRules.whole.bpl
@@ -1,7 +1,8 @@
-// the outcome of init is that: no rule to handle src tuple in ATL spec will return null, or not allocated yet.
+
 procedure init_tar_model();
 modifies $tarHeap;
 ensures  (forall $o: ref :: $o == null || !read($tarHeap, $o, alloc));
+
 
 
 procedure SM2SM_matchAll() returns ();
@@ -26,6 +27,7 @@ getTarsBySrcs(Seq#Singleton(sm1)) !=null
   free ensures $HeapSucc(old($tarHeap), $tarHeap);
   free ensures $HeapSucc(old($linkHeap), $linkHeap);
   free ensures surj_tar_model($srcHeap, $tarHeap);
+
 
 
 
@@ -58,6 +60,7 @@ getTarsBySrcs(Seq#Singleton(rs1)) !=null
 
 
 
+
 procedure IS2IS_matchAll() returns ();
   requires (forall is1: ref :: is1!=null && read($srcHeap, is1, alloc) && dtype(is1) <: HSM$InitialState 
  ==>
@@ -80,6 +83,7 @@ getTarsBySrcs(Seq#Singleton(is1)) !=null
   free ensures $HeapSucc(old($tarHeap), $tarHeap);
   free ensures $HeapSucc(old($linkHeap), $linkHeap);
   free ensures surj_tar_model($srcHeap, $tarHeap);
+
 
 
 
@@ -112,6 +116,8 @@ getTarsBySrcs(Seq#Singleton(is1)) !=null
 
 
 
+
+
 procedure T2TA_matchAll() returns ();
   requires (forall t1: ref :: t1!=null && read($srcHeap, t1, alloc) && dtype(t1) <: HSM$Transition 
  ==>
@@ -134,6 +140,7 @@ getTarsBySrcs(Seq#Singleton(t1)) !=null
   free ensures $HeapSucc(old($tarHeap), $tarHeap);
   free ensures $HeapSucc(old($linkHeap), $linkHeap);
   free ensures surj_tar_model($srcHeap, $tarHeap);
+
 
 
 
@@ -172,6 +179,7 @@ getTarsBySrcs(Seq#Build(Seq#Build(Seq#Build(Seq#Singleton(t1),src),trg),c)) !=nu
 
 
 
+
 procedure T2TC_matchAll() returns ();
   requires (forall t1,src,trg,c: ref :: t1!=null && read($srcHeap, t1, alloc) && dtype(t1) <: HSM$Transition 
  && src!=null && read($srcHeap, src, alloc) && dtype(src) <: HSM$AbstractState 
@@ -204,6 +212,7 @@ getTarsBySrcs(Seq#Build(Seq#Build(Seq#Build(Seq#Singleton(t1),src),trg),c)) !=nu
 
 
 
+
 procedure SM2SM_applyAll() returns();
   requires surj_tar_model($srcHeap, $tarHeap);
   requires (forall sm1: ref :: sm1!=null && read($srcHeap, sm1, alloc) && dtype(sm1) <: HSM$StateMachine 
@@ -222,11 +231,11 @@ getTarsBySrcs(Seq#Singleton(sm1)) !=null
 read($tarHeap, getTarsBySrcs(Seq#Singleton(sm1)), FSM$StateMachine.name) == read($srcHeap, sm1, HSM$StateMachine.name));
 
 
-
 // Frame property
   ensures (forall<alpha> $o: ref, $f: Field alpha :: 
 	!read(old($tarHeap), $o, alloc) ==>
-		 ( read($tarHeap, $o, $f) == read(old($tarHeap), $o, $f)));
+		 ( read($tarHeap, $o, $f) == read(old($tarHeap), $o, $f))
+	  || (dtype($o) == class._System.array));
   ensures (forall<alpha> $o: ref, $f: Field alpha :: 
 	$o != null && read(old($tarHeap), $o, alloc) ==>
 		(Seq#Length(getTarsBySrcs_inverse($o)) == 1 && dtype(Seq#Index(getTarsBySrcs_inverse($o), 0)) <: HSM$StateMachine && ( dtype($o) <: FSM$StateMachine && ($f == FSM$StateMachine.name))) 
@@ -256,11 +265,11 @@ read($tarHeap, getTarsBySrcs(Seq#Singleton(rs1)), FSM$AbstractState.name) == rea
 read($tarHeap, getTarsBySrcs(Seq#Singleton(rs1)), FSM$AbstractState.stateMachine) == getTarsBySrcs(Seq#Singleton(read($srcHeap, rs1, HSM$AbstractState.stateMachine))));
 
 
-
 // Frame property
   ensures (forall<alpha> $o: ref, $f: Field alpha :: 
 	!read(old($tarHeap), $o, alloc) ==>
-		 ( read($tarHeap, $o, $f) == read(old($tarHeap), $o, $f)));
+		 ( read($tarHeap, $o, $f) == read(old($tarHeap), $o, $f))
+	  || (dtype($o) == class._System.array));
   ensures (forall<alpha> $o: ref, $f: Field alpha :: 
 	$o != null && read(old($tarHeap), $o, alloc) ==>
 		(Seq#Length(getTarsBySrcs_inverse($o)) == 1 && dtype(Seq#Index(getTarsBySrcs_inverse($o), 0)) <: HSM$RegularState && ( dtype($o) <: FSM$RegularState && ($f == FSM$AbstractState.name || $f == FSM$AbstractState.stateMachine))) 
@@ -290,11 +299,11 @@ read($tarHeap, getTarsBySrcs(Seq#Singleton(is1)), FSM$AbstractState.stateMachine
 read($tarHeap, getTarsBySrcs(Seq#Singleton(is1)), FSM$AbstractState.name) == read($srcHeap, is1, HSM$AbstractState.name));
 
 
-
 // Frame property
   ensures (forall<alpha> $o: ref, $f: Field alpha :: 
 	!read(old($tarHeap), $o, alloc) ==>
-		 ( read($tarHeap, $o, $f) == read(old($tarHeap), $o, $f)));
+		 ( read($tarHeap, $o, $f) == read(old($tarHeap), $o, $f))
+	  || (dtype($o) == class._System.array));
   ensures (forall<alpha> $o: ref, $f: Field alpha :: 
 	$o != null && read(old($tarHeap), $o, alloc) ==>
 		(Seq#Length(getTarsBySrcs_inverse($o)) == 1 && dtype(Seq#Index(getTarsBySrcs_inverse($o), 0)) <: HSM$InitialState && ( dtype($o) <: FSM$InitialState && ($f == FSM$AbstractState.stateMachine || $f == FSM$AbstractState.name))) 
@@ -324,11 +333,11 @@ read($tarHeap, getTarsBySrcs(Seq#Singleton(is1)), FSM$AbstractState.stateMachine
 read($tarHeap, getTarsBySrcs(Seq#Singleton(is1)), FSM$AbstractState.name) == read($srcHeap, is1, HSM$AbstractState.name));
 
 
-
 // Frame property
   ensures (forall<alpha> $o: ref, $f: Field alpha :: 
 	!read(old($tarHeap), $o, alloc) ==>
-		 ( read($tarHeap, $o, $f) == read(old($tarHeap), $o, $f)));
+		 ( read($tarHeap, $o, $f) == read(old($tarHeap), $o, $f))
+	  || (dtype($o) == class._System.array));
   ensures (forall<alpha> $o: ref, $f: Field alpha :: 
 	$o != null && read(old($tarHeap), $o, alloc) ==>
 		(Seq#Length(getTarsBySrcs_inverse($o)) == 1 && dtype(Seq#Index(getTarsBySrcs_inverse($o), 0)) <: HSM$InitialState && ( dtype($o) <: FSM$RegularState && ($f == FSM$AbstractState.stateMachine || $f == FSM$AbstractState.name))) 
@@ -366,11 +375,11 @@ read($tarHeap, getTarsBySrcs(Seq#Singleton(t1)), FSM$Transition.source) == getTa
 read($tarHeap, getTarsBySrcs(Seq#Singleton(t1)), FSM$Transition.target) == getTarsBySrcs(Seq#Singleton(read($srcHeap, t1, HSM$Transition.target))));
 
 
-
 // Frame property
   ensures (forall<alpha> $o: ref, $f: Field alpha :: 
 	!read(old($tarHeap), $o, alloc) ==>
-		 ( read($tarHeap, $o, $f) == read(old($tarHeap), $o, $f)));
+		 ( read($tarHeap, $o, $f) == read(old($tarHeap), $o, $f))
+	  || (dtype($o) == class._System.array));
   ensures (forall<alpha> $o: ref, $f: Field alpha :: 
 	$o != null && read(old($tarHeap), $o, alloc) ==>
 		(Seq#Length(getTarsBySrcs_inverse($o)) == 1 && dtype(Seq#Index(getTarsBySrcs_inverse($o), 0)) <: HSM$Transition && ( dtype($o) <: FSM$Transition && ($f == FSM$Transition.label || $f == FSM$Transition.stateMachine || $f == FSM$Transition.source || $f == FSM$Transition.target))) 
@@ -423,11 +432,11 @@ read($tarHeap, getTarsBySrcs(Seq#Build(Seq#Build(Seq#Build(Seq#Singleton(t1),src
 read($tarHeap, getTarsBySrcs(Seq#Build(Seq#Build(Seq#Build(Seq#Singleton(t1),src),trg),c)), FSM$Transition.target) == getTarsBySrcs(Seq#Singleton(trg)));
 
 
-
 // Frame property
   ensures (forall<alpha> $o: ref, $f: Field alpha :: 
 	!read(old($tarHeap), $o, alloc) ==>
-		 ( read($tarHeap, $o, $f) == read(old($tarHeap), $o, $f)));
+		 ( read($tarHeap, $o, $f) == read(old($tarHeap), $o, $f))
+	  || (dtype($o) == class._System.array));
   ensures (forall<alpha> $o: ref, $f: Field alpha :: 
 	$o != null && read(old($tarHeap), $o, alloc) ==>
 		(Seq#Length(getTarsBySrcs_inverse($o)) == 4 && dtype(Seq#Index(getTarsBySrcs_inverse($o), 0)) <: HSM$Transition && dtype(Seq#Index(getTarsBySrcs_inverse($o), 1)) <: HSM$CompositeState && dtype(Seq#Index(getTarsBySrcs_inverse($o), 2)) <: HSM$AbstractState && dtype(Seq#Index(getTarsBySrcs_inverse($o), 3)) <: HSM$AbstractState && ( dtype($o) <: FSM$Transition && ($f == FSM$Transition.label || $f == FSM$Transition.stateMachine || $f == FSM$Transition.source || $f == FSM$Transition.target))) 
@@ -480,11 +489,11 @@ read($tarHeap, getTarsBySrcs(Seq#Build(Seq#Build(Seq#Build(Seq#Singleton(t1),src
 read($tarHeap, getTarsBySrcs(Seq#Build(Seq#Build(Seq#Build(Seq#Singleton(t1),src),trg),c)), FSM$Transition.target) == getTarsBySrcs(Seq#Singleton(c)));
 
 
-
 // Frame property
   ensures (forall<alpha> $o: ref, $f: Field alpha :: 
 	!read(old($tarHeap), $o, alloc) ==>
-		 ( read($tarHeap, $o, $f) == read(old($tarHeap), $o, $f)));
+		 ( read($tarHeap, $o, $f) == read(old($tarHeap), $o, $f))
+	  || (dtype($o) == class._System.array));
   ensures (forall<alpha> $o: ref, $f: Field alpha :: 
 	$o != null && read(old($tarHeap), $o, alloc) ==>
 		(Seq#Length(getTarsBySrcs_inverse($o)) == 4 && dtype(Seq#Index(getTarsBySrcs_inverse($o), 0)) <: HSM$Transition && dtype(Seq#Index(getTarsBySrcs_inverse($o), 1)) <: HSM$AbstractState && dtype(Seq#Index(getTarsBySrcs_inverse($o), 2)) <: HSM$CompositeState && dtype(Seq#Index(getTarsBySrcs_inverse($o), 3)) <: HSM$InitialState && ( dtype($o) <: FSM$Transition && ($f == FSM$Transition.label || $f == FSM$Transition.stateMachine || $f == FSM$Transition.source || $f == FSM$Transition.target))) 
